WIP: FSM abstractions

SSA/Experimental/Bits/Fast/FiniteStateMachine.lean
@@ -13,278 +13,398 @@ open Sum
 section FSM
 variable {σ β σ' β' : Type} {γ : β → Type}
 
-/-- An `arity` indexed product of Booleans. -/
-def BoolProd (arity : Type) : Type := arity → Bool
-
-def BoolProd.append (x : BoolProd σ) (y : BoolProd β) : BoolProd (Sum σ β) :=
-  fun a => match a with
-  | inl a => x a
-  | inr b => y b
+namespace BitVec
 
 @[simp]
-theorem BoolProd.append_inl (x : BoolProd σ) (y : BoolProd β) (a : σ) :
-    (x.append y) (inl a) = x a := rfl
+theorem getLsbD_append_left (x : BitVec v) (y : BitVec w) (i : Nat)
+    (h : ¬(i < w)) :
+    getLsbD (x ++ y) i = x.getLsbD (i - w) := by
+  simp [getLsbD_append, h]
 
 @[simp]
-theorem BoolProd.append_inr (x : BoolProd σ) (y : BoolProd β) (b : β) :
-    (x.append y) (inr b) = y b := rfl
+theorem getLsbD_append_right (x : BitVec v) (y : BitVec w) (i : Nat)
+    (h : i < w) :
+    getLsbD (x ++ y) i = y.getLsbD i := by
+  simp [getLsbD_append, h]
+
+/-- `appendVector` appends a family of `n` bitvectors, each of which might have
+a different width, together into a bitvector whose length is the sum of lengths
+-/
+def appendVector {ws : Fin n → Nat} (xs : (i : Fin n) → BitVec (ws i)) :
+    BitVec (∑ i, ws i) :=
+  match n with
+  | 0   => 0#_
+  | n+1 =>
+    let x := xs 0
+    (x ++ (appendVector (fun i => xs i.succ))).cast <| by
+      simp [Finset.sum]
+
+/-- Construct a bitvector from a function that maps `i : Fin w` to the
+`i`-th least significant bit -/
+def ofFnLsb (f : Fin w → Bool) : BitVec w :=
+  match w with
+  | 0   => 0#0
+  | _+1 => concat (ofFnLsb (f ∘ Fin.succ)) (f 0)
+
+@[simp] lemma getElem_ofFnLsb (f : Fin w → Bool) (i : Fin w) :
+    (ofFnLsb f)[i.val] = f i := by
+  sorry
+
+end BitVec
+
+namespace Fin
+
+def addToSum (i : Fin (x + y)) : Fin x ⊕ Fin y :=
+  if h : i < y then
+    .inr ⟨i, h⟩
+  else
+    .inl (i.subNat y <| by simp_all)
+
+@[simp] abbrev addInl (i : Fin x) : Fin (x + y) := castAdd y i
+@[simp] abbrev addInr (i : Fin y) : Fin (x + y) := natAdd x i
+
+def addElim (f : Fin x → α) (g : Fin y → α) : Fin (x + y) → α :=
+  fun i => Sum.elim f g (addToSum i)
+
+def sumOfSigma {f : α → Nat} [Fintype α] (i : Σ a, Fin (f a)) : Fin (∑ a, f a) :=
+  sorry
+
+def sumToSigma {f : α → Nat} [Fintype α] (i : Fin (∑ a, f a)) : Σ a, Fin (f a) :=
+  sorry
+
+end Fin
+
+/-- An `n`-ary product of `Bitstream`s. -/
+def BitStreamProd (n : Nat) : Type := Fin n → BitStream
+
+namespace BitStreamProd
+
+/-- Return the `i`-th stream of `x` -/
+def nthStream (x : BitStreamProd n) (i : Fin n) : BitStream := x i
+
+/-- Get the `i`th least significant bit of each constituent stream -/
+def getLsbs (xs : BitStreamProd n) (i : Nat) : BitVec n :=
+  BitVec.ofFnLsb fun j => xs j i
+
+/-- Get the least significant bit of each constituent stream -/
+def heads (xs : BitStreamProd n) : BitVec n :=
+  BitVec.ofFnLsb fun i => (xs i).head
+
+/-- Drop the least significant bit from each constituent stream,
+returning an n-ary product of each streams tail  -/
+def tails (xs : BitStreamProd n) : BitStreamProd n :=
+  fun i => (xs i).tail
+
+def castLE (h : n ≤ m) : BitStreamProd m → BitStreamProd n :=
+  (· ∘ Fin.castLE h)
+
+section Lemmas
+
+@[simp] lemma getElem_heads (xs : BitStreamProd n) (i : Fin n) :
+    xs.heads[i.val] = (xs i).head := by
+  simp [heads]
+
+@[simp] lemma getElem_getLsbs (xs : BitStreamProd n) (i : Nat) (j : Fin n) :
+    (xs.getLsbs i)[j.val] = xs j i := by
+  simp [getLsbs]
+
+end Lemmas
+
+end BitStreamProd
 
 /--
-Morally, a function from (BoolProd σ) to (BoolProd β), but the function is represented
-by mapping each output `(b : β)` to a circuit that computes the output bit `b` from the input bits `(a : σ)`.
+`CircuitProd vars n` is a collection of `n` Boolean Circuits, each of which can
+refer to at most `vars` variables.
+
+This morally represents a function from `BitVec vars`
+(i.e., an assignment of a single bit per variable),
+to a `BitVec n` (where each circuit computes a single bit of the output).
+See `CircuitProd.eval`.
 -/
-def CircuitProd (σ : Type) (β : Type)  : Type := β  → Circuit σ
+def CircuitProd (vars n : Nat) : Type := Fin n → Circuit (Fin vars)
 
-/-- A circuitProd can be evaluated to map σ product of booleans to a β product of booleans. -/
-def CircuitProd.eval (x : CircuitProd σ β) (y : BoolProd σ) : BoolProd β  :=
-  fun a => (x a).eval y
+namespace CircuitProd
 
-/-- A 'arity' indexed product of `Bitstream`s. -/
-def BitStreamProd (arity : Type) : Type := arity → BitStream
 
-def BitStreamProd.nthStream (x : BitStreamProd arity) (i : arity) : BitStream := x i
-def BitStreamProd.nthBits (x : BitStreamProd arity) (n : Nat) : BoolProd arity :=
-  fun i => (x i) n
+/-- Evaluate a `CircuitProd vars n` to the function `BitVec vars → BitVec n`
+it represents.
 
-def BitStreamProd.head (x : BitStreamProd arity) : BoolProd arity :=
-  fun i => (x i).head
+By convention, we use Little Endian order, which is to say, the `i`th circuit
+will compute the `i`-th least significant bit of the output, and the variable
+with index `i` derives it's assignment from the `i`-th least signicant bit of
+the input.
+-/
+def eval {vars n : Nat}
+    (circuit : CircuitProd vars n) (assignment : BitVec vars) :
+    BitVec n :=
+  BitVec.ofFnLsb fun i =>
+    (circuit i).eval assignment.getLsb'
 
-def BitStreamProd.tail (x : BitStreamProd arity) : BitStreamProd arity :=
-  fun a => (x a).tail
+@[simp] lemma getLsbD_eval (c : CircuitProd vars n) (assignment : BitVec vars)
+    (i : Fin n) :
+    (c.eval assignment)[i.val]
+    = (c i).eval assignment.getLsb' := by
+  simp [eval]
 
-/-- `FSM n` represents a function `BitStream → ⋯ → BitStream → BitStream`,
-where `n` is the number of `BitStream` arguments,
+instance : Subsingleton (CircuitProd n 0) :=
+  inferInstanceAs (Subsingleton (Fin 0 → _))
+
+end CircuitProd
+
+/-- `FSM arity` represents a function `BitStream → ⋯ → BitStream → BitStream`,
+where `arity` is the number of `BitStream` arguments,
 as a finite state machine.
 -/
-structure FSM (arity : Type) : Type 1 :=
+structure FSM (arity : Nat) : Type 1 :=
   /--
-  The arity of the (finite) type `σ` (for `s`tate) determines how many bits the
-  internal carry state of this FSM has -/
-  ( σ  : Type ) -- Why is σ also not an index?
-  [ i : Fintype σ ]
-  [ dec_eq : DecidableEq σ ]
-  /--
-  `initCarry` is the value of the initial internal carry state.
-  It maps each `σ` to a bit, thus it is morally a bitvector where the width is the arity of `σ`
+  `stateWidth` is the number of bits the state has
   -/
-  ( initCarry : σ → Bool )
+  (stateWidth : Nat)
   /--
-  `nextBitCirc` is a family of Boolean circuits,
-  which may refer to the current input bits *and* the current state bits
-  as free variables in the circuit.
-
-  `nextBitCirc none` computes the current output bit.
-  `nextBitCirc (some a)`, computes the *one* bit of the new state that corresponds to `a : σ`. -/
-  (currentOutCircuit : Circuit (σ ⊕ arity) ) -- given the current state, and the arguments, compute the output
-  (nextStateFnCircuit : CircuitProd (σ ⊕ arity) σ ) -- For the new state, to compute the bit `(a : σ)`, given the circuit that computes this bit from the current state and the arguments.
-
-attribute [instance] FSM.i FSM.dec_eq
-
-namespace FSM
-
-
-/-- The state of FSM `p` is given by a function from `p.σ` to `Bool`.
-
-Note that `p.σ` is assumed to be a finite type, so `p.State` is morally
-a finite bitvector whose width is given by the arity of `p.σ` -/
-abbrev State (p : FSM arity): Type := BoolProd p.σ
-
-def State.appendInput {p : FSM arity} (s : p.State) (x : BoolProd arity) :
-    BoolProd (p.σ ⊕ arity) :=
-  fun a => match a with
-  | inl a => s a
-  | inr b => x b
-
-/-- the current otuput of the FSM-/
-def outBit {p : FSM arity} (state : p.State) (input : BoolProd arity) : Bool :=
-  (p.currentOutCircuit).eval (state.appendInput input)
-
-
-end FSM
+  `initialState` is the initial state.
+  -/
+  (initialState : BitVec stateWidth)
+  /--
+  `outCircuit` is a single Boolean circuit,
+  which will compute the output bit of the current state,
+  given the current state and input bits.
+  -/
+  (outCircuit : Circuit (Fin <| stateWidth + arity))
+  /--
+  `nextStateCircuit` is a uniform family of `stateWidth` Boolean circuits,
+  where each circuit computes one bit of the next state,
+  given the current state and input bits.
+  -/
+  (nextStateCircuits : CircuitProd (stateWidth + arity) stateWidth)
 
 namespace FSM
 
-variable {arity : Type} (p : FSM arity)
+/-- A `State` of FSM `p` is just a bitvector with `p.stateWidth` bits -/
+abbrev State (p : FSM arity) : Type := BitVec p.stateWidth
 
-/-- The next state function, whieh evalutes the next state, given the current state and the input. -/
-def nextState (s : p.State) (input : BoolProd arity) : p.State :=
-  p.nextStateFnCircuit.eval (s.appendInput input)
+@[deprecated BitVec.append]
+def appendInput {p : FSM arity} (s : BitVec p.stateWidth) (x : BitVec arity) :
+    BitVec (p.stateWidth + arity) :=
+  s ++ x
+
+variable {arity : Nat} (p : FSM arity)
+
+/-- Return the output bit of FSM `p`, given the current state and input bits. -/
+@[simp]
+def outBit (state : p.State) (input : BitVec arity) : Bool :=
+  (p.outCircuit).eval (state ++ input).getLsb'
+
+/-- Return the next state of FSM `p`, given the current state and input bits. -/
+@[simp]
+def nextState (s : p.State) (input : BitVec arity) : p.State :=
+  p.nextStateCircuits.eval (s ++ input)
 
 /-- `p.next state in` computes both the next state bits and the output bit,
 where `state` are the *current* state bits, and `in` are the current input bits. -/
-def next (carry : p.State) (inputBits : BoolProd arity) : p.State × Bool :=
-    let newState : p.State  := p.nextState carry inputBits
-    let outBit : Bool       := p.outBit carry inputBits
+@[simp]
+def next (state : p.State) (inputBits : BitVec arity) : p.State × Bool :=
+    let newState := p.nextState state inputBits
+    let outBit   := p.outBit state inputBits
     (newState, outBit)
 
-
+-- TODO: document this
 def outputStreamAux (s₀ : p.State) (inputStream : BitStreamProd arity) : BitStream := fun n =>
   match n with
-  | 0 => outBit s₀ inputStream.head
-  | n+1 => outputStreamAux (nextState p s₀ (inputStream.head)) inputStream.tail n
+  | 0 => p.outBit s₀ inputStream.heads
+  | n+1 => outputStreamAux (nextState p s₀ (inputStream.heads)) inputStream.tails n
 
 @[simp]
 theorem outputStreamAux_zero (s₀ : p.State) (inputStream : BitStreamProd arity) :
-    outputStreamAux p s₀ inputStream 0 = outBit s₀ (inputStream.nthBits 0) := rfl
+    outputStreamAux p s₀ inputStream 0 = p.outBit s₀ (inputStream.getLsbs 0) := rfl
 
 @[simp]
 theorem outputStreamAux_succ (s₀ : p.State) (inputStream : BitStreamProd arity) (n : ℕ) :
     outputStreamAux p s₀ inputStream (n+1) =
-    outputStreamAux p (p.nextState s₀ (inputStream.head)) inputStream.tail n := by rfl
+    outputStreamAux p (p.nextState s₀ (inputStream.heads)) inputStream.tails n := by rfl
 
-
+/--
+A `StateStream` w.r.t. FSM `p` is an infinite stream of `p.State`s
+-/
 def StateStream (p : FSM arity) := ℕ → p.State
 
-/-- `p.carryStream inputStream` computes the stream of carries, from the stream of inputs -/
-def carryStream (inputStream : BitStreamProd arity) : p.StateStream := fun n =>
-  match n with
-  | 0 => p.initCarry
-  | n+1 => (p.nextState (carryStream inputStream n) (inputStream.nthBits n))
+/-- `p.stateStream` is the stream of states of FSM `p`,
+for a given product of input streams.
+
+That is, it is the stream that starts with `p.initialState`,
+and evolves according to `p.nextState`. -/
+def stateStream (p : FSM arity) (xs : BitStreamProd arity) : p.StateStream
+  | 0 => p.initialState
+  | n+1 => (p.nextState (p.stateStream xs n) (xs.getLsbs n))
 
 @[simp]
-theorem carryStream_zero (inputStream : BitStreamProd arity) : p.carryStream inputStream 0 = p.initCarry := rfl
+theorem stateStream_zero (xs : BitStreamProd arity) :
+    p.stateStream xs 0 = p.initialState := rfl
 
 @[simp]
-theorem carryStream_succ (inputStream : BitStreamProd arity) (n : Nat) :
-    p.carryStream inputStream (n+1) =
-    p.nextState (p.carryStream inputStream n) (inputStream.nthBits n) := rfl
+theorem stateStream_succ (inputStream : BitStreamProd arity) (n : Nat) :
+    p.stateStream inputStream (n+1)
+    = p.nextState (p.stateStream inputStream n) (inputStream.getLsbs n) :=
+  rfl
 
+-- /-- `eval p` morally gives the function `BitStream → ... → BitStream` represented by FSM `p` -/
+-- def eval (xs : BitStreamProd arity) : BitStream :=
+--   p.outputStreamAux p.initialState xs
 
-/-- `eval p` morally gives the function `BitStream → ... → BitStream` represented by FSM `p` -/
-def eval (x : BitStreamProd arity) : BitStream :=
-  p.outputStreamAux p.initCarry x
-
-def eval'Corec (input : BitStreamProd arity × p.State) :
-    (BitStreamProd arity × p.State) × Bool := -- (fun ⟨x, (carry : p.State)⟩ =>
-  let x := input.1
-  let carry := input.2
-  let x_head  := x.head -- (x · |>.head)
-  let next    := p.next carry x_head
-  let x_tail  :=  x.tail -- (x · |>.tail)
+def eval.next (xs : BitStreamProd arity × p.State) :
+    (BitStreamProd arity × p.State) × Bool := -- (fun ⟨x, (state : p.State)⟩ =>
+  let x       := xs.1
+  let state   := xs.2
+  let x_head  := x.heads
+  let next    := p.next state x_head
+  let x_tail  := x.tails
   ((x_tail, next.fst), next.snd)
 
 /-- `eval'` is an alternative definition of `eval`, written in terms of corecursion.  -/
-def eval' (x : BitStreamProd arity) : BitStream :=
-  BitStream.corec (eval'Corec p) (x, (p.initCarry : p.State))
+def eval (x : BitStreamProd arity) : BitStream :=
+  BitStream.corec (eval.next p) (x, p.initialState)
 
+-- /--
+-- Generalized hypothesis that shows how the output stream and
+-- its corecursive definition evolve with an arbitrary input state.
+-- -/
+-- theorem eval_eq_eval'_aux (i : Nat) :
+--     (p.outputStreamAux state x) i = (BitStream.corec (eval'Corec p) (x, state)) i := by
+--   induction i generalizing state x
+--   case zero => rfl
+--   case succ i ih =>
+--     simp [outputStreamAux, eval'Corec, BitStream.corec_succ]
+--     rw [← ih]
+--     rfl
+
+-- /-- Show that the two definitions of evaluation are equivalent. -/
+-- theorem eval_eq_eval' : p.eval x = p.eval' x := by
+--   funext i
+--   apply eval_eq_eval'_aux
+
+/-- `p.withInitialState s` yields an FSM with `s` as the initial state -/
+def withInitialState (p : FSM arity) (s : p.State) : FSM arity :=
+  { p with initialState := s }
+
+theorem eval_withInitialState_succ
+    (p : FSM arity) (c : p.State) (xs : BitStreamProd arity) (n : ℕ) :
+    (p.withInitialState c).eval xs (n+1) =
+      (p.withInitialState (p.nextState c xs.heads)).eval (xs.tails) n := by
+  simp [eval, withInitialState, next]; rfl
+
+
+-- /-- `p.changeVars f` changes the arity of an `FSM`.
+-- The function `f` determines how the new input bits map to the input expected by `p` -/
+-- def changeVars {newArity : Nat} (changeVars : Fin arity → Fin newArity) :
+--     FSM newArity :=
+--   let map (x : BitVec newArity) : BitVec arity :=
+--     BitVec.ofFnLsb (fun j => x[changeVars j])
+--   { p with
+--     outCircuit := p.outCircuit.map _
+--     -- nextBitCirc := fun a => (p.nextBitCirc a).map (Sum.map id changeVars) }
+
+-- open Fin in
+-- def composeUnary (p : FSM 1) (q : FSM n) : FSM n where
+--   stateWidth := p.stateWidth + q.stateWidth
+--   initialState := p.initialState ++ q.initialState
+--   outCircuit := p.outCircuit.bind <| addCases
+--     (fun i => Circuit.var true (addInl <| addInl i))
+--     (fun _ => q.outCircuit.map fun j =>
+--       j.natAdd p.stateWidth |>.cast (by ac_rfl)
+--     )
+--   nextStateCircuits :=
+--    addCases
+--     (fun i => (p.nextStateCircuits i).bind <| )
+--     _
+--     -- p.nextStateCircuits
+
+open Fin in
 /--
-Generalized hypothesis that shows how the output stream and
-its corecursive definition evolve with an arbitrary input state.
--/
-theorem eval_eq_eval'_aux (i : Nat) :
-    (p.outputStreamAux state x) i = (BitStream.corec (eval'Corec p) (x, state)) i := by
-  induction i generalizing state x
-  case zero => rfl
-  case succ i ih =>
-    simp [outputStreamAux, eval'Corec, BitStream.corec_succ]
-    rw [← ih]
-    rfl
+Given an FSM `p` of some `arity`,
+and a family of `arity` FSMs `qᵢ`,
+whose (possibly differing) arities are bounded by `newArity`,
+we can compose `p` with `qᵢ` yielding a single FSM of arity `newArity`.
 
-/-- Show that the two definitions of evaluation are equivalent. -/
-theorem eval_eq_eval' : p.eval x = p.eval' x := by
-  funext i
-  apply eval_eq_eval'_aux
+The input of the composed FSM is given to the FSMs `qᵢ`, each of which computes
+a single bit of the input that is then given to `p`. -/
+def compose {newArity : Nat} {qArity : Fin arity → Nat}
+    (arityLE : ∀ (a : Fin arity), qArity a ≤ newArity)
+    (q : (i : Fin arity) → FSM (qArity i)) :
+    FSM newArity :=
+  let qOutCircuit (i : Fin arity) :=
+    (q i).outCircuit.map <| Fin.addElim
+      (fun j => (addInl (addInr (sumOfSigma ⟨i, j⟩))))
+      (fun j => addInr (j.castLE (arityLE i)))
+  { stateWidth    := p.stateWidth + (∑ i, (q i).stateWidth),
+    initialState  := p.initialState ++ (BitVec.appendVector (q · |>.initialState))
+    outCircuit :=
+      open Fin in
+      p.outCircuit.bind <| addCases
+        (fun i => Circuit.var true <| (addInl <| addInl i))
+        qOutCircuit
+    nextStateCircuits :=
+      open Fin in
+      addCases
+       (fun i => (p.nextStateCircuits i).bind <| addCases
+          (fun j => Circuit.var true (addInl (addInl j)))
+          qOutCircuit
+       )
+       (fun i =>
+        let ⟨i, j⟩ := i.sumToSigma
+        ((q i).nextStateCircuits j).map <| addCases
+          (fun k => addInl (addInr (sumOfSigma ⟨_, k⟩)))
+          (fun k => addInr (k.castLE <| arityLE i))
+      )
+  }
 
-/-- `p.changeInitCarry c` yields an FSM with `c` as the initial state -/
-def changeInitCarry (p : FSM arity) (c : BoolProd p.σ) : FSM arity :=
-  { p with initCarry := c }
+#check FSM.stateStream
 
-theorem eval_changeInitCarry_succ
-    (p : FSM arity) (c : p.σ → Bool) (x : BitStreamProd arity) (n : ℕ) :
-    (p.changeInitCarry c).eval x (n+1) =
-      (p.changeInitCarry (p.next c (fun a => x a 0)).1).eval
-        (fun a i => x a (i+1)) n := by
-  rw [eval, carry_changeInitCarry_succ]
-  simp [eval, changeInitCarry, next]
-
-/-- `p.changeVars f` changes the arity of an `FSM`.
-The function `f` determines how the new input bits map to the input expected by `p` -/
-def changeVars {arity2 : Type} (changeVars : arity → arity2) : FSM arity2 :=
-  { p with nextBitCirc := fun a => (p.nextBitCirc a).map (Sum.map id changeVars) }
-
-/--
-Given an FSM `p` of arity `n`,
-a family of `n` FSMs `qᵢ` of posibly different arities `mᵢ`,
-and given yet another arity `m` such that `mᵢ ≤ m` for all `i`,
-we can compose `p` with `qᵢ` yielding a single FSM of arity `m`,
-such that each FSM `qᵢ` computes the `i`th bit that is fed to the FSM `p`. -/
-def compose [Fintype arity] [DecidableEq arity]
-    (new_arity : Type)        -- `new_arity` is the resulting arity
-    (q_arity : arity → Type)  -- `q_arityₐ` is the arity of FSM `qₐ`
-    (vars : ∀ (a : arity), q_arity a → new_arity)
-    -- ^^ `vars` is the function that tells us, for each FSM `qₐ`,
-    --     which bits of the final `new_arity` corresponds to the `q_arityₐ` bits expected by `qₐ`
-    (q : ∀ (a : arity), FSM (q_arity a)) : -- `q` gives the FSMs to be composed with `p`
-    FSM new_arity :=
-  { σ := p.σ ⊕ (Σ a, (q a).σ),
-    i := by letI := p.i; infer_instance,
-    dec_eq := by
-      letI := p.dec_eq
-      letI := fun a => (q a).dec_eq
-      infer_instance,
-    initCarry := Sum.elim p.initCarry (λ x => (q x.1).initCarry x.2),
-    nextBitCirc := λ a =>
-      match a with
-      | none => (p.nextBitCirc none).bind
-        (Sum.elim
-          (fun a => Circuit.var true (inl (inl a)))
-          (fun a => ((q a).nextBitCirc none).map
-            (Sum.elim (fun d => (inl (inr ⟨a, d⟩))) (fun q => inr (vars a q)))))
-      | some (inl a) =>
-        (p.nextBitCirc (some a)).bind
-          (Sum.elim
-            (fun a => Circuit.var true (inl (inl a)))
-            (fun a => ((q a).nextBitCirc none).map
-            (Sum.elim (fun d => (inl (inr ⟨a, d⟩))) (fun q => inr (vars a q)))))
-      | some (inr ⟨x, y⟩) =>
-          ((q x).nextBitCirc (some y)).map
-            (Sum.elim
-              (fun a => inl (inr ⟨_, a⟩))
-              (fun a => inr (vars x a))) }
-
-lemma carry_compose [Fintype arity] [DecidableEq arity]
-    (new_arity : Type)
-    (q_arity : arity → Type)
-    (vars : ∀ (a : arity), q_arity a → new_arity)
-    (q : ∀ (a : arity), FSM (q_arity a))
-    (x : new_BitStreamProd arity) : ∀ (n : ℕ),
-    (p.compose new_arity q_arity vars q).carry x n =
-      let z := p.carry (λ a => (q a).eval (fun i => x (vars _ i))) n
-      Sum.elim z (fun a => (q a.1).carry (fun t => x (vars _ t)) n a.2)
-  | 0 => by simp [carry, compose]
-  | n+1 => by
-      rw [carry, carry_compose _ _ _ _ _ n]
-      ext y
-      cases y
-      · simp [carry, next, compose, Circuit.eval_bind, eval]
+lemma stateStream_compose {newArity : Nat} {qArity : Fin arity → Nat}
+    (arityLE : ∀ (i : Fin arity), qArity i ≤ newArity)
+    (q : ∀ (i : Fin arity), FSM (qArity i))
+    (xs : BitStreamProd newArity)
+    (n : Nat) :
+    (p.compose arityLE q).stateStream xs n =
+      let pState := p.stateStream (fun i =>
+        (q i).eval (fun j => xs <| j.castLE (arityLE _))) n
+      let qState : BitVec (∑ i, (q i).stateWidth) :=
+        BitVec.appendVector fun i =>
+          ((q i).stateStream (xs.castLE <| arityLE _) n)
+      pState ++ qState := by
+  induction n with
+  | zero => simp [stateStream, compose]
+  | succ n ih =>
+      rw [stateStream, ih]
+      ext (y : Fin (_ + _))
+      cases y using Fin.addCases
+      · simp [stateStream, next, compose, Circuit.eval_bind, eval]
         congr
-        ext z
-        cases z
-        · simp
-        · simp [Circuit.eval_map, carry]
+        ext (z : Fin (_ + _))
+        cases z using Fin.addCases
+        · simp;
+          sorry
+        · simp [Circuit.eval_map, stateStream]
           congr
-          ext s
-          cases s
-          · simp
-          · simp
-      · simp [Circuit.eval_map, carry, compose, eval, carry, next]
+          ext (s : Fin (_ + _))
+          cases s using Fin.addCases
+          · simp; sorry
+          · simp; sorry
+      · simp [Circuit.eval_map, stateStream, compose, eval, next]
         congr
-        ext z
-        cases z
-        · simp
-        · simp
+        ext (z : Fin (_ + _))
+        cases z using Fin.addCases
+        · simp; sorry
+        · simp; sorry
 
 /-- Evaluating a composed fsm is equivalent to composing the evaluations of the constituent FSMs -/
-lemma eval_compose [Fintype arity] [DecidableEq arity]
-    (new_arity : Type)
-    (q_arity : arity → Type)
-    (vars : ∀ (a : arity), q_arity a → new_arity)
-    (q : ∀ (a : arity), FSM (q_arity a))
-    (x : new_BitStreamProd arity) :
-    (p.compose new_arity q_arity vars q).eval x =
-      p.eval (λ a => (q a).eval (fun i => x (vars _ i))) := by
+lemma eval_compose {newArity : Nat} {qArity : Fin arity → Nat}
+    (arityLE : ∀ (i : Fin arity), qArity i ≤ newArity)
+    (q : ∀ (i : Fin arity), FSM (qArity i))
+    (x : BitStreamProd newArity) :
+    (p.compose arityLE q).eval x =
+      p.eval (λ a => (q a).eval (fun i => x (i.castLE <| arityLE _))) := by
   ext n
-  rw [eval, carry_compose, eval]
+  stop
+  rw [eval, stateStream_compose, eval]
   simp [compose, next, Circuit.eval_bind]
   congr
   ext a
@@ -297,72 +417,95 @@ lemma eval_compose [Fintype arity] [DecidableEq arity]
   simp
   simp
 
-def v0 : Fin 2 → BitStream
-  | ⟨0, _⟩ => fun n => n % 2 = 0
-  | ⟨1, _⟩ => fun n => n % 2 = 1
+/-!
+## Concrete FSMs
+From here on out, we start to implement various operations as concrete FSMs
+-/
 
-def and : FSM Bool :=
-  { σ := Empty,
-    initCarry := Empty.elim,
-    nextStateFnCircuit := fun a => a.elim,
-    currentOutCircuit :=
-      (Circuit.and
-        (Circuit.var true (inr true))
-        (Circuit.var true (inr false))) }
+/-! ### Bitwise operations -/
 
-@[simp] lemma eval_and (x : Bool → BitStream) : and.eval x = (x true) &&& (x false) := by
-  ext n; cases n <;> simp [and, eval, next]
+/-- `mapCircuit` lifts a Boolean circuit into a stateless FSM -/
+def mapCircuit (c : Circuit (Fin n)) : FSM n where
+  stateWidth := 0
+  initialState := 0#0
+  outCircuit := c.map (Fin.cast <| by ac_rfl)
+  nextStateCircuits := Fin.elim0
 
-def or : FSM Bool :=
-  { σ := Empty,
-    initCarry := Empty.elim,
-    nextBitCirc := fun a => a.elim
-      (Circuit.or
-        (Circuit.var true (inr true))
-        (Circuit.var true (inr false))) Empty.elim }
+@[simp] lemma eval_mapCircuit (c : Circuit (Fin n)) (xs : BitStreamProd n) :
+    (mapCircuit c).eval xs = (fun n => c.eval fun j => (xs.getLsbs n)[j.val]) := by
+  funext m
+  simp only [eval, mapCircuit]
+  induction m generalizing xs
+  case zero =>
+    simp [eval.next, next, BitVec.zero_width_append _, BitStream.head]
+  case succ m ih =>
+
+    simp [eval.next]
+    specialize ih xs.tails
+
+    simp at ih
+    rw [ih (xs.tails)]
+
+
+
+def and : FSM 2 :=
+  mapCircuit (Circuit.and
+    (Circuit.var true 1)
+    (Circuit.var true 0))
+
+@[simp] lemma eval_and (xs : BitStreamProd 2) :
+    and.eval x = (xs 1) &&& (xs 0) := by
+  ext n;
+  -- stop
+  cases n <;> simp [mapCircuit, and, eval, next]
+
+def or : FSM 2 :=
+  mapCircuit (Circuit.or
+    (Circuit.var true 1)
+    (Circuit.var true 0))
 
 @[simp] lemma eval_or (x : Bool → BitStream) : or.eval x = (x true) ||| (x false) := by
   ext n; cases n <;> simp [and, eval, next]
 
-def xor : FSM Bool :=
-  { σ := Empty,
-    initCarry := Empty.elim,
-    nextBitCirc := fun a => a.elim
-      (Circuit.xor
-        (Circuit.var true (inr true))
-        (Circuit.var true (inr false))) Empty.elim }
+def xor : FSM 2 :=
+  mapCircuit (Circuit.xor
+    (Circuit.var true 1)
+    (Circuit.var true 0))
 
-@[simp] lemma eval_xor (x : Bool → BitStream) : xor.eval x = (x true) ^^^ (x false) := by
-  ext n; cases n <;> simp [and, eval, next]
+@[simp] lemma eval_xor (xs : BitStreamProd 2) :
+    xor.eval xs = (xs 1) ^^^ (xs 0) := by
+  ext n; stop cases n <;> simp [and, eval, next]
 
-def add : FSM Bool :=
-  { σ := Unit,
-    initCarry := λ _ => false,
-    nextBitCirc := fun a =>
-      match a with
-      | some () =>
-             (Circuit.var true (inr true)  &&& Circuit.var true (inr false))
-             ||| (Circuit.var true (inr true)  &&& Circuit.var true (inl ()))
-             ||| (Circuit.var true (inr false) &&& Circuit.var true (inl ()))
-      | none => Circuit.var true (inr true) ^^^
-                Circuit.var true (inr false) ^^^
-                Circuit.var true (inl ()) }
+/-! ### Arithmetic -/
 
-/-- The internal carry state of the `add` FSM agrees with
+def add : FSM 2 where
+  stateWidth := 1
+  initialState := 0#1
+  outCircuit :=
+    Circuit.var true 0
+    ^^^ Circuit.var true 1
+    ^^^ Circuit.var true 2
+  nextStateCircuits _ :=
+    (Circuit.var true 2 &&& Circuit.var true 1)
+    ||| (Circuit.var true 2  &&& Circuit.var true 0)
+    ||| (Circuit.var true 1 &&& Circuit.var true 0)
+
+/-- The internal state of the `add` FSM agrees with
 the carry bit of addition as implemented on bitstreams -/
-theorem carry_add_succ (x : Bool → BitStream) (n : ℕ) :
-    add.carry x (n+1) =
-      fun _ => (BitStream.addAux (x true) (x false) n).2 := by
-  ext a; obtain rfl : a = () := rfl
+theorem carry_add_succ (xs : BitStreamProd 2) (n : ℕ) :
+    add.stateStream xs (n+1)
+    = BitVec.ofBool ((BitStream.addAux (xs 1) (xs 0) n).2) := by
+  ext (a : Fin 1)
+  obtain rfl : a = (0 : Fin 1) := Fin.fin_one_eq_zero a
   induction n with
   | zero      =>
-    simp [carry, BitStream.addAux, next, add, BitVec.adcb]
+    simp [stateStream, BitStream.addAux, next, add, BitVec.adcb]
   | succ n ih =>
     unfold carry
     simp [next, ih, Circuit.eval, BitStream.addAux, BitVec.adcb]
 
-@[simp] theorem carry_zero (x : BitStreamProd arity) : carry p x 0 = p.initCarry := rfl
-@[simp] theorem initCarry_add : add.initCarry = (fun _ => false) := rfl
+@[simp] theorem carry_zero (x : BitStreamProd arity) : carry p x 0 = p.initialState := rfl
+@[simp] theorem initialState_add : add.initialState = (fun _ => false) := rfl
 
 @[simp] lemma eval_add (x : Bool → BitStream) : add.eval x = (x true) + (x false) := by
   ext n
@@ -378,7 +521,7 @@ given that we can reduce both those operations to just addition and bitwise comp
 
 def sub : FSM Bool :=
   { σ := Unit,
-    initCarry := fun _ => false,
+    initialState := fun _ => false,
     nextBitCirc := fun a =>
       match a with
       | some () =>
@@ -409,7 +552,7 @@ theorem eval_sub (x : Bool → BitStream) : sub.eval x = (x true) - (x false) :=
 def neg : FSM Unit :=
   { σ := Unit,
     i := by infer_instance,
-    initCarry := λ _ => true,
+    initialState := λ _ => true,
     nextBitCirc := fun a =>
       match a with
       | some () => Circuit.var false (inr ()) &&& Circuit.var true (inl ())
@@ -433,7 +576,7 @@ theorem carry_neg (x : Unit → BitStream) : ∀ (n : ℕ), neg.carry x (n+1) =
 
 def not : FSM Unit :=
   { σ := Empty,
-    initCarry := Empty.elim,
+    initialState := Empty.elim,
     nextBitCirc := fun _ => Circuit.var false (inr ()) }
 
 @[simp] lemma eval_not (x : Unit → BitStream) : not.eval x = ~~~(x ()) := by
@@ -441,7 +584,7 @@ def not : FSM Unit :=
 
 def zero : FSM (Fin 0) :=
   { σ := Empty,
-    initCarry := Empty.elim,
+    initialState := Empty.elim,
     nextBitCirc := fun _ => Circuit.fals }
 
 @[simp] lemma eval_zero (x : Fin 0 → BitStream) : zero.eval x = BitStream.zero := by
@@ -450,7 +593,7 @@ def zero : FSM (Fin 0) :=
 def one : FSM (Fin 0) :=
   { σ := Unit,
     i := by infer_instance,
-    initCarry := λ _ => true,
+    initialState := λ _ => true,
     nextBitCirc := fun a =>
       match a with
       | some () => Circuit.fals
@@ -469,7 +612,7 @@ def one : FSM (Fin 0) :=
 def negOne : FSM (Fin 0) :=
   { σ := Empty,
     i := by infer_instance,
-    initCarry := Empty.elim,
+    initialState := Empty.elim,
     nextBitCirc := fun _ => Circuit.tru }
 
 @[simp] lemma eval_negOne (x : Fin 0 → BitStream) : negOne.eval x = BitStream.negOne := by
@@ -477,7 +620,7 @@ def negOne : FSM (Fin 0) :=
 
 def ls (b : Bool) : FSM Unit :=
   { σ := Unit,
-    initCarry := fun _ => b,
+    initialState := fun _ => b,
     nextBitCirc := fun x =>
       match x with
       | none => Circuit.var true (inl ())
@@ -501,7 +644,7 @@ theorem carry_ls (b : Bool) (x : Unit → BitStream) : ∀ (n : ℕ),
 def var (n : ℕ) : FSM (Fin (n+1)) :=
   { σ := Empty,
     i := by infer_instance,
-    initCarry := Empty.elim,
+    initialState := Empty.elim,
     nextBitCirc := λ _ => Circuit.var true (inr (Fin.last _)) }
 
 @[simp] lemma eval_var (n : ℕ) (x : Fin (n+1) → BitStream) : (var n).eval x = x (Fin.last n) := by
@@ -509,7 +652,7 @@ def var (n : ℕ) : FSM (Fin (n+1)) :=
 
 def incr : FSM Unit :=
   { σ := Unit,
-    initCarry := fun _ => true,
+    initialState := fun _ => true,
     nextBitCirc := fun x =>
       match x with
       | none => (Circuit.var true (inr ())) ^^^ (Circuit.var true (inl ()))
@@ -532,7 +675,7 @@ theorem carry_incr (x : Unit → BitStream) : ∀ (n : ℕ),
 def decr : FSM Unit :=
   { σ := Unit,
     i := by infer_instance,
-    initCarry := λ _ => true,
+    initialState := λ _ => true,
     nextBitCirc := fun x =>
       match x with
       | none => (Circuit.var true (inr ())) ^^^ (Circuit.var true (inl ()))
@@ -554,7 +697,7 @@ theorem carry_decr (x : Unit → BitStream) : ∀ (n : ℕ), decr.carry x (n+1) 
 
 theorem evalAux_eq_zero_of_set {arity : Type _} (p : FSM arity)
     (R : Set (p.σ → Bool)) (hR : ∀ x s, (p.next s x).1 ∈ R → s ∈ R)
-    (hi : p.initCarry ∉ R) (hr1 : ∀ x s, (p.next s x).2 = true → s ∈ R)
+    (hi : p.initialState ∉ R) (hr1 : ∀ x s, (p.next s x).2 = true → s ∈ R)
     (x : BitStreamProd arity) (n : ℕ) : p.eval x n = false ∧ p.carry x n ∉ R := by
   simp (config := {singlePass := true}) only [← not_imp_not] at hR hr1
   simp only [Bool.not_eq_true] at hR hr1
@@ -568,7 +711,7 @@ theorem evalAux_eq_zero_of_set {arity : Type _} (p : FSM arity)
 
 theorem eval_eq_zero_of_set {arity : Type _} (p : FSM arity)
     (R : Set (p.σ → Bool)) (hR : ∀ x s, (p.next s x).1 ∈ R → s ∈ R)
-    (hi : p.initCarry ∉ R) (hr1 : ∀ x s, (p.next s x).2 = true → s ∈ R) :
+    (hi : p.initialState ∉ R) (hr1 : ∀ x s, (p.next s x).2 = true → s ∈ R) :
     p.eval = fun _ _ => false := by
   ext x n
   rw [eval]
@@ -576,7 +719,7 @@ theorem eval_eq_zero_of_set {arity : Type _} (p : FSM arity)
 
 def repeatBit : FSM Unit where
   σ := Unit
-  initCarry := fun () => false
+  initialState := fun () => false
   nextBitCirc := fun _ =>
     .or (.var true <| .inl ()) (.var true <| .inr ())
 
@@ -730,7 +873,7 @@ If not, we produce an infinite sequence of `1`.
 -/
 def and : FSM Bool :=
   { σ := Unit,
-    initCarry := fun _ => false,
+    initialState := fun _ => false,
     nextBitCirc := fun a =>
       match a with
       | some () =>
@@ -751,7 +894,7 @@ If not, we produce a `1`.
 -/
 def or : FSM Bool :=
   { σ := Unit,
-    initCarry := fun _ => false,
+    initialState := fun _ => false,
     nextBitCirc := fun a =>
       match a with
       | some () =>
@@ -800,7 +943,7 @@ theorem decideIfZeroAux_wf {σ : Type _} [Fintype σ] [DecidableEq σ]
 
 def decideIfZerosAux {arity : Type _} [DecidableEq arity]
     (p : FSM arity) (c : Circuit p.σ) : Bool :=
-  if c.eval p.initCarry
+  if c.eval p.initialState
   then false
   else
     have c' := (c.bind (p.nextBitCirc ∘ some)).fst
@@ -818,14 +961,14 @@ def decideIfZeros {arity : Type _} [DecidableEq arity]
 theorem decideIfZerosAux_correct {arity : Type _} [DecidableEq arity]
     (p : FSM arity) (c : Circuit p.σ)
     (hc : ∀ s, c.eval s = true →
-      ∃ m y, (p.changeInitCarry s).eval y m = true)
+      ∃ m y, (p.withInitialState s).eval y m = true)
     (hc₂ : ∀ (x : arity → Bool) (s : p.σ → Bool),
       (FSM.next p s x).snd = true → Circuit.eval c s = true) :
     decideIfZerosAux p c = true ↔ ∀ n x, p.eval x n = false := by
   rw [decideIfZerosAux]
   split_ifs with h
   · simp
-    exact hc p.initCarry h
+    exact hc p.initialState h
   · dsimp
     split_ifs with h'
     · simp only [true_iff]
@@ -847,7 +990,7 @@ theorem decideIfZerosAux_correct {arity : Type _} [DecidableEq arity]
       · rcases hc _ hx with ⟨m, y, hmy⟩
         use (m+1)
         use fun a i => Nat.casesOn i x (fun i a => y a i) a
-        rw [FSM.eval_changeInitCarry_succ]
+        rw [FSM.eval_withInitialState_succ]
         rw [← hmy]
         simp only [FSM.next, Nat.rec_zero, Nat.rec_add_one]
       · exact hc _ h
@@ -864,7 +1007,7 @@ theorem decideIfZeros_correct {arity : Type _} [DecidableEq arity]
     intro s x h
     use 0
     use (fun a _ => x a)
-    simpa [FSM.eval, FSM.changeInitCarry, FSM.next, FSM.carry]
+    simpa [FSM.eval, FSM.withInitialState, FSM.next, FSM.carry]
   · simp only [Circuit.eval_fst]
     intro x s h
     use x
